repeat/AddI.v
@@ -21,17 +21,17 @@ Module AddI. Section AddI.
       fb <- ((cenv.(CEnv.id2blk) AddHdr.succ)?);;
       ccallU RepeatHdr.repeat [Vptr (fb, 0%Z); Vint n; Vint m].
 
-  Definition fnsems (genv: GEnv.t) :=
-    [(AddHdr.succ, (wmask_all, scopes, cfunU succ));
-     (AddHdr.add, (wmask_all, scopes, cfunU (add (CEnv.load_genv genv))))].
+  Definition fnsems (genv: GEnv.t) : alist (option string) (fnsem_type (option fspec * fbody)):=
+    [(Some AddHdr.succ, (false, wmask_all, scopes, (None, cfunU succ)));
+     (Some AddHdr.add, (false, wmask_all, scopes, (None, cfunU (add (CEnv.load_genv genv)))))].
 
-  Program Definition Mod (genv: GEnv.t) : PMod.t := {|
-    PMod.scopes := scopes;
-    PMod.fnsems := fnsems genv;
-    PMod.initial_st := [];
+  Program Definition Mod (genv: GEnv.t) : SMod.t := {|
+    SMod.scopes := scopes;
+    SMod.fnsems := fnsems genv;
+    SMod.initial_st := [];
   |}.
   Solve All Obligations with prove_scope.
   Next Obligation. prove_nodup. Qed.
 
-  Definition t (genv: GEnv.t) : HMod.t := Seal.sealing CRIS (PMod.to_hmod (Mod genv)).
+  Definition t (genv: GEnv.t) : HMod.t := Seal.sealing CRIS (SMod.to_hmod sp_none (Mod genv)).
 End AddI. End AddI.
